reorganize swap, bring down to a few cheats

examples/riscv/swap/swap_propScript.sml
@@ -1,210 +1,38 @@
 open HolKernel boolLib Parse bossLib;
 
-open distribute_generic_stuffLib;
+open markerTheory;
 
 open bir_programSyntax bir_program_labelsTheory;
 open bir_immTheory bir_valuesTheory bir_expTheory;
 open bir_tsTheory bir_bool_expTheory bir_programTheory;
 
 open bir_riscv_backlifterTheory;
-open bir_riscv_extrasTheory;
 open bir_backlifterLib;
 open bir_compositionLib;
 
-open bir_wpLib bir_wp_expLib;
-open bir_wpTheory bir_htTheory;
-open bir_wp_interfaceLib;
+open bir_lifting_machinesTheory;
+open bir_typing_expTheory;
+open bir_htTheory;
 
 open tutorial_smtSupportLib;
 
-open bir_symbTheory birs_auxTheory;
-open HolBACoreSimps;
-open bir_program_transfTheory;
-open bir_symbLib;
-
 open total_program_logicTheory;
 open total_ext_program_logicTheory;
-open symb_prop_transferTheory;
 
 open jgmt_rel_bir_contTheory;
 
-open birs_stepLib;
+open pred_setTheory;
+
+open program_logicSimps;
+
+open bir_env_oldTheory;
+open bir_program_varsTheory;
 
 open swapTheory;
-
-open swap_symb_execTheory;
-
-open distribute_generic_stuffTheory;
+open swap_specTheory;
+open swap_symb_transfTheory;
 
 val _ = new_theory "swap_prop";
-
-Definition swap_mem_spec_def:
- swap_mem_spec ms =
- let ms'_mem8 = (riscv_mem_store_dword (ms.c_gpr ms.procID 0w)
-   (riscv_mem_load_dword ms.MEM8 (ms.c_gpr ms.procID 1w)) ms.MEM8)
- in
-   (riscv_mem_store_dword (ms.c_gpr ms.procID 1w)
-    (riscv_mem_load_dword ms.MEM8 (ms.c_gpr ms.procID 0w)) ms'_mem8)
-End
-
-Definition swap_spec_output_def:
- swap_spec_output ms : riscv_state = ms with MEM8 := swap_mem_spec ms
-End
-
-Definition swap_spec_def:
- swap_spec ms ms' : bool = (ms'.MEM8 = swap_mem_spec ms)
-End
-
-(* --------------- *)
-(* RISC-V contract *)
-(* --------------- *)
-
-Definition riscv_swap_pre_def:
- riscv_swap_pre x y xv yv (m : riscv_state) =
-  (m.c_gpr m.procID 10w = x /\
-   riscv_mem_load_dword m.MEM8 x = xv /\
-   m.c_gpr m.procID 11w = y /\
-   riscv_mem_load_dword m.MEM8 y = yv)
-End
-
-Definition riscv_swap_post_def:
- riscv_swap_post x y xv yv (m : riscv_state) =
-  (riscv_mem_load_dword m.MEM8 x = yv /\
-   riscv_mem_load_dword m.MEM8 y = xv)
-End
-
-val bir_swap_pre_tm = bslSyntax.bandl [
- mem_addrs_aligned_prog_disj_tm "x10",
- mem_addrs_aligned_prog_disj_tm "x11",
- ``BExp_BinPred
-    BIExp_Equal
-    (BExp_Den (BVar "x10" (BType_Imm Bit64)))
-    (BExp_Const (Imm64 x))``,
- ``BExp_BinPred
-      BIExp_Equal
-      (BExp_Load
-       (BExp_Den (BVar "MEM8" (BType_Mem Bit64 Bit8)))
-       (BExp_Den (BVar "x10" (BType_Imm Bit64)))
-       BEnd_LittleEndian Bit64)
-      (BExp_Const (Imm64 xv))``,
- ``BExp_BinPred
-     BIExp_Equal
-     (BExp_Den (BVar "x11" (BType_Imm Bit64)))
-     (BExp_Const (Imm64 y))``,
- ``BExp_BinPred
-    BIExp_Equal
-     (BExp_Load
-      (BExp_Den (BVar "MEM8" (BType_Mem Bit64 Bit8)))
-      (BExp_Den (BVar "x11" (BType_Imm Bit64)))
-      BEnd_LittleEndian Bit64)
-     (BExp_Const (Imm64 yv))`` 
-];
-
-Definition bir_swap_pre_def:
-  bir_swap_pre x y xv yv : bir_exp_t =
-   ^bir_swap_pre_tm
-End
-
-Definition bir_swap_post_def:
- bir_swap_post x y xv yv : bir_exp_t = 
-  BExp_BinExp BIExp_And
-   (BExp_BinPred
-    BIExp_Equal
-    (BExp_Load
-     (BExp_Den (BVar "MEM8" (BType_Mem Bit64 Bit8)))
-     (BExp_Const (Imm64 x))
-     BEnd_LittleEndian Bit64)
-    (BExp_Const (Imm64 yv)))
-   (BExp_BinPred
-    BIExp_Equal
-    (BExp_Load
-     (BExp_Den (BVar "MEM8" (BType_Mem Bit64 Bit8)))
-     (BExp_Const (Imm64 y))
-     BEnd_LittleEndian Bit64)
-    (BExp_Const (Imm64 xv)))
-End
-
-val bir_swap_pre = ``bir_swap_pre``;
-val bir_swap_post = ``bir_swap_post``;
-
-(* ----------------------------------- *)
-(* Connecting RISC-V and BIR contracts *)
-(* ----------------------------------- *)
-
-Theorem swap_riscv_pre_imp_bir_pre_thm[local]:
- bir_pre_riscv_to_bir
-  (riscv_swap_pre pre_x10 pre_x11 pre_x10_mem_deref pre_x11_mem_deref)
-  (bir_swap_pre pre_x10 pre_x11 pre_x10_mem_deref pre_x11_mem_deref)
-Proof
- cheat
-QED
-
-Theorem swap_riscv_post_imp_bir_post_thm[local]:
- !ls. bir_post_bir_to_riscv
-   (riscv_swap_post pre_x10 pre_x11 pre_x10_mem_deref pre_x11_mem_deref)
-   (\l. (bir_swap_post pre_x10 pre_x11 pre_x10_mem_deref pre_x11_mem_deref))
-   ls
-Proof
- rw [bir_post_bir_to_riscv_def,riscv_swap_post_def,bir_swap_post_def,riscv_mem_load_dword_def] >>
- Cases_on `bs` >>
- Cases_on `b0` >>
- FULL_SIMP_TAC (std_ss++holBACore_ss) [
-  bir_envTheory.bir_env_read_def, bir_envTheory.bir_env_check_type_def,
-  bir_envTheory.bir_env_lookup_type_def, bir_envTheory.bir_env_lookup_def,bir_eval_bin_pred_def] >>
- cheat
-QED
-
-(* ------------------------------- *)
-(* BIR symbolic execution analysis *)
-(* ------------------------------- *)
-
-val (sys_i, L_s, Pi_f) = (symb_sound_struct_get_sysLPi_fun o concl) swap_symb_analysis_thm;
-
-Definition swap_analysis_L_def:
- swap_analysis_L = ^(L_s)
-End
-
-val birs_state_init_lbl = ``<|bpc_label := BL_Address (Imm64 0x00w); bpc_index := 0|>``;
-val birs_state_end_lbl = (snd o dest_eq o concl o EVAL) ``bir_block_pc (BL_Address (Imm64 0x14w))``;
-
-Theorem swap_analysis_L_NOTIN_thm[local]:
-  (^birs_state_end_lbl) NOTIN swap_analysis_L
-Proof
-  EVAL_TAC
-QED
-
-(* ........................... *)
-(* ........................... *)
-(* ........................... *)
-
-val birs_state_init_pre = ``birs_state_init_pre_GEN ^birs_state_init_lbl swap_birenvtyl
- (mk_bsysprecond (bir_swap_pre pre_x10 pre_x11 pre_x10_mem_deref pre_x11_mem_deref) swap_birenvtyl)``;
-
-val swap_bsysprecond_thm = (computeLib.RESTR_EVAL_CONV [``birs_eval_exp``] THENC birs_stepLib.birs_eval_exp_CONV)
- ``mk_bsysprecond (bir_swap_pre pre_x10 pre_x11 pre_x10_mem_deref pre_x11_mem_deref) swap_birenvtyl``;
-
-(*
-Theorem birs_state_init_pre_EQ_thm:
-  ^((snd o dest_comb) sys_i) = ^birs_state_init_pre
-Proof
-  REWRITE_TAC [birs_state_init_pre_GEN_def, mk_bsysprecond_def, swap_bsysprecond_thm] >>
-  CONV_TAC (computeLib.RESTR_EVAL_CONV [``birs_eval_exp``] THENC birs_stepLib.birs_eval_exp_CONV)
-QED
-
-val swap_analysis_thm =
-  REWRITE_RULE [birs_state_init_pre_EQ_thm, GSYM bir_swap_prog_def] swap_symb_analysis_thm;
-*)
-
-Theorem bir_cont_swap:
- bir_cont bir_swap_prog bir_exp_true (BL_Address (Imm64 0x00w))
-  {BL_Address (Imm64 0x14w)} {}
-  (bir_swap_pre pre_x10 pre_x11 pre_x10_mem_deref pre_x11_mem_deref)
-  (\l. if l = BL_Address (Imm64 0x14w)
-       then (bir_swap_post pre_x10 pre_x11 pre_x10_mem_deref pre_x11_mem_deref)
-       else bir_exp_false)
-Proof
- cheat
-QED
 
 (* ---------------------------------- *)
 (* Backlifting BIR contract to RISC-V *)
