examples/riscv/swap/swap_specScript.sml
@@ -1,0 +1,165 @@
+open HolKernel boolLib Parse bossLib;
+
+open markerTheory;
+
+open distribute_generic_stuffLib;
+
+open bir_programSyntax bir_program_labelsTheory;
+open bir_immTheory bir_valuesTheory bir_expTheory;
+open bir_tsTheory bir_bool_expTheory bir_programTheory;
+
+open bir_riscv_backlifterTheory;
+open bir_backlifterLib;
+open bir_riscv_extrasTheory;
+open bir_compositionLib;
+
+open bir_lifting_machinesTheory;
+open bir_typing_expTheory;
+open bir_htTheory;
+
+open tutorial_smtSupportLib;
+open bir_symbLib;
+
+open bir_symbTheory birs_auxTheory;
+open HolBACoreSimps;
+open bir_program_transfTheory;
+
+open total_program_logicTheory;
+open total_ext_program_logicTheory;
+open symb_prop_transferTheory;
+
+open jgmt_rel_bir_contTheory;
+
+open bir_symbTheory;
+open birs_stepLib;
+open bir_symb_sound_coreTheory;
+open symb_recordTheory;
+open symb_interpretTheory;
+
+open pred_setTheory;
+
+open program_logicSimps;
+
+open bir_env_oldTheory;
+open bir_program_varsTheory;
+
+open distribute_generic_stuffTheory;
+
+open swapTheory;
+
+val _ = new_theory "swap_spec";
+
+Definition swap_mem_spec_def:
+ swap_mem_spec ms =
+ let ms'_mem8 = (riscv_mem_store_dword (ms.c_gpr ms.procID 0w)
+   (riscv_mem_load_dword ms.MEM8 (ms.c_gpr ms.procID 1w)) ms.MEM8)
+ in
+   (riscv_mem_store_dword (ms.c_gpr ms.procID 1w)
+    (riscv_mem_load_dword ms.MEM8 (ms.c_gpr ms.procID 0w)) ms'_mem8)
+End
+
+Definition swap_spec_output_def:
+ swap_spec_output ms : riscv_state = ms with MEM8 := swap_mem_spec ms
+End
+
+Definition swap_spec_def:
+ swap_spec ms ms' : bool = (ms'.MEM8 = swap_mem_spec ms)
+End
+
+(* --------------- *)
+(* RISC-V contract *)
+(* --------------- *)
+
+Definition riscv_swap_pre_def:
+ riscv_swap_pre x y xv yv (m : riscv_state) =
+  (m.c_gpr m.procID 10w = x /\
+   riscv_mem_load_dword m.MEM8 x = xv /\
+   m.c_gpr m.procID 11w = y /\
+   riscv_mem_load_dword m.MEM8 y = yv)
+End
+
+Definition riscv_swap_post_def:
+ riscv_swap_post x y xv yv (m : riscv_state) =
+  (riscv_mem_load_dword m.MEM8 x = yv /\
+   riscv_mem_load_dword m.MEM8 y = xv)
+End
+
+val bir_swap_pre_tm = bslSyntax.bandl [
+ mem_addrs_aligned_prog_disj_tm "x10",
+ mem_addrs_aligned_prog_disj_tm "x11",
+ ``BExp_BinPred
+    BIExp_Equal
+    (BExp_Den (BVar "x10" (BType_Imm Bit64)))
+    (BExp_Const (Imm64 x))``,
+ ``BExp_BinPred
+      BIExp_Equal
+      (BExp_Load
+       (BExp_Den (BVar "MEM8" (BType_Mem Bit64 Bit8)))
+       (BExp_Den (BVar "x10" (BType_Imm Bit64)))
+       BEnd_LittleEndian Bit64)
+      (BExp_Const (Imm64 xv))``,
+ ``BExp_BinPred
+     BIExp_Equal
+     (BExp_Den (BVar "x11" (BType_Imm Bit64)))
+     (BExp_Const (Imm64 y))``,
+ ``BExp_BinPred
+    BIExp_Equal
+     (BExp_Load
+      (BExp_Den (BVar "MEM8" (BType_Mem Bit64 Bit8)))
+      (BExp_Den (BVar "x11" (BType_Imm Bit64)))
+      BEnd_LittleEndian Bit64)
+     (BExp_Const (Imm64 yv))`` 
+];
+
+Definition bir_swap_pre_def:
+  bir_swap_pre x y xv yv : bir_exp_t =
+   ^bir_swap_pre_tm
+End
+
+Definition bir_swap_post_def:
+ bir_swap_post x y xv yv : bir_exp_t = 
+  BExp_BinExp BIExp_And
+   (BExp_BinPred
+    BIExp_Equal
+    (BExp_Load
+     (BExp_Den (BVar "MEM8" (BType_Mem Bit64 Bit8)))
+     (BExp_Const (Imm64 x))
+     BEnd_LittleEndian Bit64)
+    (BExp_Const (Imm64 yv)))
+   (BExp_BinPred
+    BIExp_Equal
+    (BExp_Load
+     (BExp_Den (BVar "MEM8" (BType_Mem Bit64 Bit8)))
+     (BExp_Const (Imm64 y))
+     BEnd_LittleEndian Bit64)
+    (BExp_Const (Imm64 xv)))
+End
+
+(* ----------------------------------- *)
+(* Connecting RISC-V and BIR contracts *)
+(* ----------------------------------- *)
+
+Theorem swap_riscv_pre_imp_bir_pre_thm:
+ bir_pre_riscv_to_bir
+  (riscv_swap_pre pre_x10 pre_x11 pre_x10_mem_deref pre_x11_mem_deref)
+  (bir_swap_pre pre_x10 pre_x11 pre_x10_mem_deref pre_x11_mem_deref)
+Proof
+ cheat
+QED
+
+Theorem swap_riscv_post_imp_bir_post_thm:
+ !ls. bir_post_bir_to_riscv
+   (riscv_swap_post pre_x10 pre_x11 pre_x10_mem_deref pre_x11_mem_deref)
+   (\l. (bir_swap_post pre_x10 pre_x11 pre_x10_mem_deref pre_x11_mem_deref))
+   ls
+Proof
+ rw [bir_post_bir_to_riscv_def,riscv_swap_post_def,bir_swap_post_def,riscv_mem_load_dword_def] >>
+ Cases_on `bs` >>
+ Cases_on `b0` >>
+ FULL_SIMP_TAC (std_ss++holBACore_ss) [
+  bir_envTheory.bir_env_read_def, bir_envTheory.bir_env_check_type_def,
+  bir_envTheory.bir_env_lookup_type_def, bir_envTheory.bir_env_lookup_def,bir_eval_bin_pred_def] >>
+ cheat
+QED
+
+val _ = export_theory ();
